IRStepObj.thy
@@ -32,8 +32,7 @@ type_synonym Program = "Signature \<rightharpoonup> IRGraph"
 text_raw \<open>\EndSnip\<close>
 
 inductive step :: "IRGraph \<Rightarrow> (ID \<times> MapState \<times> DynamicHeap) \<Rightarrow> (ID \<times> MapState \<times> DynamicHeap) \<Rightarrow> bool"
-  ("_ \<turnstile> _ \<rightarrow> _" 55)
-  where
+  ("_ \<turnstile> _ \<rightarrow> _" 55) for g where
 
   SequentialNode:
   "\<lbrakk>is_sequential_node (kind g nid);
@@ -126,7 +125,7 @@ theorem "stepDet":
    "(g \<turnstile> (nid,m,h) \<rightarrow> next) \<Longrightarrow>
    (\<forall> next'. ((g \<turnstile> (nid,m,h) \<rightarrow> next') \<longrightarrow> next = next'))"
 proof (induction rule: "step.induct")
-  case (SequentialNode g nid "next" m h)
+  case (SequentialNode nid "next" m h)
   have notif: "\<not>(is_IfNode (kind g nid))"
     using SequentialNode.hyps(1) is_sequential_node.simps 
     by (metis is_IfNode_def)
@@ -149,7 +148,7 @@ proof (induction rule: "step.induct")
   show ?case using SequentialNode step.cases
     by (smt (verit) is_IfNode_def is_LoadFieldNode_def is_NewInstanceNode_def is_RefNode_def is_StoreFieldNode_def prod.inject)
 next
-  case (IfNode g nid cond tb fb m val "next" h)
+  case (IfNode nid cond tb fb m val "next" h)
   then have notseq: "\<not>(is_sequential_node (kind g nid))"
     using is_sequential_node.simps isAbstractMergeNodeType.simps
     by (simp add: IfNode.hyps(1))
@@ -159,7 +158,7 @@ next
   from notseq notend show ?case using IfNode evalDet
     by (smt (verit) IRNode.distinct(871) IRNode.distinct(891) IRNode.distinct(909) IRNode.distinct(923) IRNode.inject(11) Pair_inject step.cases)
 next
-  case (EndNodes g nid merge i phis inputs m vs m' h)
+  case (EndNodes nid merge i phis inputs m vs m' h)
   have notseq: "\<not>(is_sequential_node (kind g nid))"
     using EndNodes.hyps(1) isAbstractEndNodeType.simps is_sequential_node.simps 
     by (metis is_EndNode.elims(2) is_LoopEndNode_def)
@@ -182,7 +181,7 @@ next
   show ?case using EndNodes evalAllDet
     by (smt (verit) is_IfNode_def is_LoadFieldNode_def is_NewInstanceNode_def is_RefNode_def is_StoreFieldNode_def prod.inject step.cases)
 next
-  case (RefNode g nid nid' m h)
+  case (RefNode nid nid' m h)
   then have notseq: "\<not>(is_sequential_node (kind g nid))"
     using is_sequential_node.simps isAbstractMergeNodeType.simps
     by (simp add: RefNode.hyps(1))
@@ -193,7 +192,7 @@ next
   show ?case
     by (smt (z3) IRNode.distinct(1329) IRNode.distinct(1739) IRNode.distinct(1937) IRNode.distinct(923) IRNode.sel(108) RefNode.hyps fst_conv snd_conv step.cases) 
 next
-  case (NewInstanceNode g nid f obj nxt h' ref h m' m)
+  case (NewInstanceNode nid f obj nxt h' ref h m' m)
   then have notseq: "\<not>(is_sequential_node (kind g nid))"
     using is_sequential_node.simps isAbstractMergeNodeType.simps
     by (simp add: NewInstanceNode.hyps(1))
@@ -204,7 +203,7 @@ next
   show ?case using NewInstanceNode step.cases
     by (smt (z3) IRNode.distinct(1297) IRNode.distinct(1725) IRNode.distinct(1739) IRNode.distinct(891) IRNode.inject(28) fst_conv snd_conv)
 next
-  case (LoadFieldNode g nid f obj nxt m ref h v m')
+  case (LoadFieldNode nid f obj nxt m ref h v m')
   then have notseq: "\<not>(is_sequential_node (kind g nid))"
     using is_sequential_node.simps isAbstractMergeNodeType.simps
     by (simp add: LoadFieldNode.hyps(1))
@@ -215,7 +214,7 @@ next
   show ?case using LoadFieldNode step.cases
     by (smt (z3) IRNode.distinct(1297) IRNode.distinct(1315) IRNode.distinct(1329) IRNode.distinct(871) IRNode.inject(18) LoadFieldNode.hyps(1) LoadFieldNode.hyps(2) LoadFieldNode.hyps(3) LoadFieldNode.hyps(4) Pair_inject Value.inject(3) evalDet option.discI option.inject)
 next
-  case (StaticLoadFieldNode g nid f nxt h v m' m)
+  case (StaticLoadFieldNode nid f nxt h v m' m)
   then have notseq: "\<not>(is_sequential_node (kind g nid))"
     using is_sequential_node.simps isAbstractMergeNodeType.simps
     by (simp add: StaticLoadFieldNode.hyps(1))
@@ -226,7 +225,7 @@ next
   show ?case using StaticLoadFieldNode step.cases
     by (smt (z3) IRNode.distinct(1297) IRNode.distinct(1315) IRNode.distinct(1329) IRNode.distinct(871) IRNode.inject(18) Pair_inject option.discI)
 next
-  case (StoreFieldNode g nid f newval uu obj nxt m val ref h' h m')
+  case (StoreFieldNode nid f newval uu obj nxt m val ref h' h m')
   then have notseq: "\<not>(is_sequential_node (kind g nid))"
     using is_sequential_node.simps isAbstractMergeNodeType.simps
     by (simp add: StoreFieldNode.hyps(1))
@@ -237,7 +236,7 @@ next
   show ?case using StoreFieldNode step.cases
     by (smt (z3) IRNode.distinct(1315) IRNode.distinct(1725) IRNode.distinct(1937) IRNode.distinct(909) IRNode.inject(37) Pair_inject Value.inject(3) evalDet option.discI option.inject)
 next
-  case (StaticStoreFieldNode g nid f newval uv nxt m val h' h m')
+  case (StaticStoreFieldNode nid f newval uv nxt m val h' h m')
   then have notseq: "\<not>(is_sequential_node (kind g nid))"
     using is_sequential_node.simps isAbstractMergeNodeType.simps
     by (simp add: StaticStoreFieldNode.hyps(1))
